src/Language/PlutusIR/Semantics/SemanticEquivalence/CompatibilityLemmas/LamAbs.v
@@ -43,12 +43,49 @@ Proof.
          reflexivity.
 Qed.
 
+Lemma msubstA_LamAbs : forall ss x T t0 t',
+    msubstA ss (LamAbs x T t0) t' ->
+    exists t0', msubstA ss t0 t0' /\ t' = LamAbs x (msubstT ss T) t0'.
+Proof.
+  induction ss.
+  - intros. 
+    inversion H. subst.
+    exists t0.
+    split. 
+    + apply msubstA_nil.
+    + reflexivity. 
+  - intros.
+    inversion H. subst.
+    rename t'0 into t''.
+    inversion H2.
+    subst.
+    simpl.
+    edestruct IHss as [t0'' [HmsA__t0'' Heq]]; eauto.
+    subst.
+    eexists.
+    split.
+    + eapply msubstA_cons. eauto. eauto.
+    + reflexivity. 
+Qed.
+
+Lemma msubstT_TyFun : forall ss T1 T2,
+    msubstT ss (Ty_Fun T1 T2) = Ty_Fun (msubstT ss T1) (msubstT ss T2).
+Proof.
+  induction ss.
+  - reflexivity.
+  - intros.
+    simpl.
+    destruct a.
+    apply IHss.
+Qed.
+
+
 Lemma compatibility_LamAbs : forall Delta Gamma x T1 e e' T2,
     (Delta, Gamma) |-* T1 : Kind_Base ->
     LR_logically_approximate Delta (x |-> T1; Gamma) e e' T2 ->
     LR_logically_approximate Delta Gamma (LamAbs x T1 e) (LamAbs x T1 e') (Ty_Fun T1 T2).
 Proof.
-  intros Delta Gamma x T1 e e' T2 Hkind__T1 IH_LR.
+  intros Delta Gamma x T1 eb eb' T2 Hkind__T1 IH_LR.
   unfold LR_logically_approximate.
 
   split. {
@@ -64,33 +101,51 @@ Proof.
   intros k rho env env' ct ck HeqDelta HeqGamma [H_RD H_RG].
   subst.
 
-  intros e_s e'_s Hms__e_s Hms__e'_s.
+  intros e_sa e'_sa e_s e'_s.
+  intros HmsA__e_sa HmsA__e'_sa Hms__e_s Hms__e'_s.
 
   assert (Hcls1 : closed_env env) by (eapply RG_env_closed_1; eauto).
   assert (Hcls2 : closed_env env') by (eapply RG_env_closed_2; eauto).
-  destruct (msubst_LamAbs _ _ _ _ _ Hcls1 Hms__e_s) as [e_s0 [Hms__e_s0 Heq]].
-  destruct (msubst_LamAbs _ _ _ _ _ Hcls2 Hms__e'_s) as [e'_s0 [Hms__e'_s0 Heq']].
+  destruct (msubstA_LamAbs _ _ _ _ _ HmsA__e_sa) as [eb_sa [HmsA__eb_sa Heq]].
+  destruct (msubstA_LamAbs _ _ _ _ _ HmsA__e'_sa) as [eb'_sa [HmsA__eb'_sa Heq']].
+  subst.
+  destruct (msubst_LamAbs _ _ _ _ _ Hcls1 Hms__e_s) as [eb_s [Hms__eb_s Heq]].
+  destruct (msubst_LamAbs _ _ _ _ _ Hcls2 Hms__e'_s) as [eb'_s [Hms__eb'_s Heq']].
   subst.
   clear Hcls1 Hcls2.
 
-  assert (emptyContext |-+ (LamAbs x T1 e_s0) : (msubstT_rho_syn1 rho (Ty_Fun T1 T2))). {
-    Axiom skip : forall P, P.
-    apply skip.
-  }
-  assert (emptyContext |-+ (LamAbs x T1 e'_s0) : (msubstT_rho_syn2 rho (Ty_Fun T1 T2))) by apply skip.
-
-  unfold P_has_type in IH_LR.
+  unfold LR_logically_approximate in IH_LR.
 
   autorewrite with RC.
-  split; auto. split; auto.
+  split. {
+    eapply msubst_preserves_typing_1; eauto.
+    rewrite msubstT_TyFun.
+    destruct IH_LR.
+    eapply T_LamAbs.
+Abort.
+(*
+    + eauto.
+
+
+    apply skip.
+  }
+  split. {
+    apply skip.
+  }
+
   intros j Hlt__j e_f Hev__e_f.
   inversion Hev__e_f. subst.
-  exists (LamAbs x T1 e'_s0).
+  exists (LamAbs x (msubstT (msyn2 rho) T1) eb'_s).
   exists 0.
   split. {
     eapply eval_value. apply V_LamAbs.
   }
   intros.
+
+  eapply IH_LR.
+  - reflexivity.
+  - reflexivity. 
+
   inversion H1. subst.
   inversion H2. subst.
 
@@ -105,3 +160,4 @@ Proof.
   + apply V_cons; eauto.
     eapply instantiation_drop.
     apply skip.
+*)
