src/Language/PlutusIR/Semantics/SemanticEquivalence/CompatibilityLemmas/Var.v
@@ -8,31 +8,38 @@ Require Import Arith.
 
 Lemma msubst_Var : forall ss x,
     closed_env ss ->
-    value_env ss ->
     forall t',
       msubst ss (Var x) t' ->
         match lookup x ss with
-        | Datatypes.Some t => t' = t /\ value t 
+        | Datatypes.Some t => t' = t
         | None=> t' = Var x
         end.
 Proof. 
   induction ss; intros.
-  - inversion H1. subst.
+  - inversion H0. subst.
     reflexivity.
-  - inversion H1. subst.
+  - inversion H0. subst.
     simpl.
-    inversion H4; subst.
+    inversion H3; subst.
     + rewrite String.eqb_refl.
-      split.
-      * eapply msubst_closed; eauto.
-        inversion H; auto.
-      * destruct H0. 
-        assumption. 
-    + apply String.eqb_neq in H6.
-      rewrite H6.
+      eapply msubst_closed; eauto.
+      inversion H; auto.
+    + apply String.eqb_neq in H5.
+      rewrite H5.
       apply IHss; eauto.
       inversion H; auto.
-      inversion H0; auto.
+Qed.
+
+Lemma msubstA_Var : forall ss x t',
+  msubstA ss (Var x) t' ->
+  t' = Var x.
+Proof.
+  induction ss; intros.
+  - inversion H. subst.
+    reflexivity.
+  - inversion H. subst.
+    inversion H2. subst.
+    auto.
 Qed.
 
 Lemma compatibility_Var : forall Delta Gamma x T,
@@ -48,7 +55,7 @@ Proof.
   intros k rho env env' ct ck HeqDelta HeqGamma [H_RD H_RG].
   subst.
 
-  intros e_s e'_s Hms__e_s Hms__e'_s.
+  intros e_sa e'_sa e_s e'_s HmsA__e_sa HmsA__e'_sa Hms__e_s Hms__e'_s.
 
   assert (forall x, (mupdate empty ct) x = lookup x ct). {
       intros. erewrite mupdate_lookup. auto.
@@ -58,16 +65,19 @@ Proof.
 
   destruct (RG_domains_match _ _ _ _ _ H_RG _ _ Hx) as [v [v' [Hlu__v Hlu__v']]].
   destruct (RG_env_closed _ _ _ _ _ H_RG) as [Hcls__env Hcls__env'].
-  destruct (RG_env_values _ _ _ _ _ H_RG) as [Hvals__env Hvals__env'].
 
   eapply RG_RC.
   - apply H_RG.
   - apply Hx.
-  - apply msubst_Var in Hms__e_s; eauto.
+  - apply msubstA_Var in HmsA__e_sa.
+    subst.
+    apply msubst_Var in Hms__e_s; eauto.
     rewrite Hlu__v in Hms__e_s.
     destruct Hms__e_s. subst.
     assumption.
-  - apply msubst_Var in Hms__e'_s; eauto.
+  - apply msubstA_Var in HmsA__e'_sa.
+    subst.
+    apply msubst_Var in Hms__e'_s; eauto.
     rewrite Hlu__v' in Hms__e'_s.
     destruct Hms__e'_s. subst.
     assumption.
